Micro_Rust_Parser_Experiment/Parser_Impl.thy
@@ -18,4 +18,11 @@ urust_expr smoke_sfx  \<open> 1_u32 \<close>
 urust_expr smoke_unit \<open> () \<close>
 thm smoke_num_def smoke_sfx_def smoke_unit_def
 
+ML_val\<open>
+  val _ =
+    if Global_Theory.defined_fact \<^theory> "smoke_num_conformance"
+    then error "default urust_conformance_check unexpectedly generated a theorem"
+    else ()
+\<close>
+
 end
